fix printer: implemented missing functions; can now parse some small examples

theories/binary_format_tests.v
@@ -92,12 +92,26 @@ Definition empty_module := {|
 Lemma empty_module_round_trip : run_parse_module (binary_of_module empty_module) = Some empty_module.
 Proof. vm_compute. reflexivity. Qed.
 
-Definition module_42 := {|
+Definition module_type := {|
+  mod_types := cons (Tf nil (cons T_i32 nil)) nil;
+  mod_funcs := nil;
+  mod_tables := nil;
+  mod_mems := nil;
+  mod_globals := nil;
+  mod_elem := nil;
+  mod_data := nil;
+  mod_start := None;
+  mod_imports := nil;
+  mod_exports := nil;
+|}.
+
+Lemma module_type_round_trip :
+  run_parse_module (binary_of_module module_type) = Some module_type.
+Proof. vm_compute. reflexivity. Qed.
+
+Definition module_type_fun := {|
   mod_types := cons (Tf nil (cons T_i32 nil)) nil;
   mod_funcs :=
-  (*
-    let e := EConst (ConstInt32 (Wasm_int.Int32.repr (BinInt.Z.of_nat 42))) in
-    *)
     cons {| mf_type := Mk_typeidx 0; mf_locals := nil; mf_body := nil |} nil;
   mod_tables := nil;
   mod_mems := nil;
@@ -109,5 +123,25 @@ Definition module_42 := {|
   mod_exports := nil;
 |}.
 
-Lemma module_42_round_trip : run_parse_module (binary_of_module module_42) = Some module_42.
+Lemma module_type_fun_round_trip :
+  run_parse_module (binary_of_module module_type_fun) = Some module_type_fun.
+Proof. vm_compute. reflexivity. Qed.
+
+Definition module_42 := {|
+  mod_types := cons (Tf nil (cons T_i32 nil)) nil;
+  mod_funcs :=
+    let e := EConst (ConstInt32 (Wasm_int.Int32.repr (BinInt.Z.of_nat 42))) in
+    cons {| mf_type := Mk_typeidx 0; mf_locals := nil; mf_body := cons e nil |} nil;
+  mod_tables := nil;
+  mod_mems := nil;
+  mod_globals := nil;
+  mod_elem := nil;
+  mod_data := nil;
+  mod_start := None;
+  mod_imports := nil;
+  mod_exports := nil;
+|}.
+
+Lemma module_42_round_trip :
+  run_parse_module (binary_of_module module_42) = Some module_42.
 Proof. vm_compute. reflexivity. Qed.
